Rewrite of label-free (logic) language - labels as part of syntax, continued

label-free/Semantics.v
@@ -1,67 +1,69 @@
 (* TODO: imports are messed up now that there's a module *) 
 Require Import Syntax.
 Require Import Substitution.
+Require Import Metatheory.
 Require Import LibList.
 Require Import LibListSorted.
 Require Import Arith.
 
 Open Scope label_free_is5_scope.
 
-Global Reserved Notation " G '|=' Gamma '|-' M ':::' A " (at level 70).
-
-Definition Background_LF := list Context_LF.
+Global Reserved Notation " G '|=' Ctx '|-' M ':::' A " (at level 70).
 
 (* Statics *)
 
 Inductive types_LF: Background_LF -> Context_LF -> te_LF -> ty_LF -> Prop :=
 
-| t_hyp_LF: forall A G Gamma v_n
+| t_hyp_LF: forall A G w Gamma v_n
   (HT: Nth v_n Gamma A),
-  G |= Gamma |- (hyp_LF v_n) ::: A
+  G |= (w, Gamma) |- (hyp_LF v_n) ::: A
 
-| t_lam_LF: forall A B G Gamma M 
-  (HT: G |= A::Gamma |- M ::: B),
-  G |= Gamma |- (lam_LF A M) ::: A ---> B
+| t_lam_LF: forall A B G w Gamma M 
+  (HT: G |= (w, A::Gamma) |- M ::: B),
+  G |= (w, Gamma) |- (lam_LF A M) ::: A ---> B
 
-| t_appl_LF: forall A B G Gamma M N
-  (HT1: G |= Gamma |- M ::: A ---> B)
-  (HT2: G |= Gamma |- N ::: A),
-  G |= Gamma |- (appl_LF M N) ::: B
+| t_appl_LF: forall A B G Ctx M N
+  (HT1: G |= Ctx |- M ::: A ---> B)
+  (HT2: G |= Ctx |- N ::: A),
+  G |= Ctx |- (appl_LF M N) ::: B
 
-| t_box_LF: forall A G Gamma M
-  (HT: G & Gamma |= nil |- M ::: A),
-  G |= Gamma |- (box_LF M) ::: [*] A
+| t_box_LF: forall L A G Ctx M
+  (HT: forall w', w' \notin L -> 
+    G & Ctx |= (w', nil) |- M ^^ (fctx w') ::: A),
+  G |= Ctx |- box_LF M ::: [*] A
 
-| t_unbox_LF: forall A G Gamma M
-  (HT: G |= Gamma |- M ::: [*] A),
-  G |= Gamma |- unbox_LF M ::: A
+| t_unbox_LF: forall A G Ctx M
+  (HT: G |= Ctx |- M ::: [*] A),
+  G |= Ctx |- unbox_LF M ::: A
 
-| t_unbox_fetch_LF: forall A G Gamma Gamma' M
-  (HT: G & Gamma' |= Gamma |- M ::: [*] A),
-  forall G', permut (G & Gamma) G' ->
-    G' |= Gamma' |- unbox_fetch_LF M Gamma ::: A
+| t_unbox_fetch_LF: forall A G w Gamma Ctx' M
+  (HT: G & Ctx' |= (w, Gamma) |- M ::: [*] A),
+  forall G', permut (G & (w, Gamma)) G' ->
+    G' |= Ctx' |- unbox_fetch_LF (fctx w) M ::: A
 
-| t_here_LF: forall A G Gamma M
-  (HT: G |= Gamma |- M ::: A),
-  G |= Gamma |- here_LF M ::: <*> A
+| t_here_LF: forall A G Ctx M
+  (HT: G |= Ctx |- M ::: A),
+  G |= Ctx |- here_LF M ::: <*> A
 
-| t_get_here_LF: forall A G Gamma Gamma' M
-  (HT: G & Gamma' |= Gamma |- M ::: A),
-  forall G0, permut (G & Gamma) G0 -> 
-    G0 |= Gamma' |- get_here_LF M Gamma ::: <*> A
+| t_get_here_LF: forall A G w Gamma Ctx' M
+  (HT: G & Ctx' |= (w, Gamma) |- M ::: A),
+  forall G0, permut (G & (w, Gamma)) G0 -> 
+    G0 |= Ctx' |- get_here_LF (fctx w) M ::: <*> A
 
-| t_letdia_LF: forall A B G Gamma M N
-  (HT1: G |= Gamma |- M ::: <*> A)
-  (HT2: (A :: nil) :: G |= Gamma |- N ::: B),
-  G |= Gamma |- letdia_LF M N ::: B 
+| t_letdia_LF: forall L A B G Ctx M N
+  (HT1: G |= Ctx |- M ::: <*> A)
+  (HT2: forall w', w' \notin L ->
+    (w', A :: nil) :: G |= Ctx |- N ^^ (fctx w') ::: B),
+  G |= Ctx |- letdia_LF M N ::: B 
 
-| t_letdia_get_LF: forall A B G Gamma Gamma' M N
-  (HT1: G & Gamma' |= Gamma |- M ::: <*> A)
-  (HT2: (A :: nil) :: G & Gamma |= Gamma' |- N ::: B),
-  forall G0, permut (G & Gamma) G0 -> 
-    G0 |= Gamma' |- letdia_get_LF M N Gamma ::: B
+| t_letdia_get_LF: forall L A B G w Gamma Ctx' M N
+  (HT1: G & Ctx' |= (w, Gamma) |- M ::: <*> A)
+  (HT2: forall w', w' \notin L ->
+    (w', (A :: nil)) :: G & (w, Gamma) |= Ctx' |- N ^^ (fctx w') ::: B),
+  forall G0, permut (G & (w, Gamma)) G0 -> 
+    G0 |= Ctx' |- letdia_get_LF (fctx w) M N ::: B
 
-where " G '|=' Gamma '|-' M ':::' A " := (types_LF G Gamma M A) : label_free_is5_scope.
+where " G '|=' Ctx '|-' M ':::' A " := (types_LF G Ctx M A) : label_free_is5_scope.
 
 (* Dynamics *)
 
@@ -69,535 +71,141 @@ Inductive value_LF: te_LF -> Prop :=
 | val_lam_LF: forall A M, value_LF (lam_LF A M)
 | val_box_LF: forall M, value_LF (box_LF M)
 | val_here_LF: forall M, value_LF M -> value_LF (here_LF M)
-| val_get_here_LF: forall M Gamma, value_LF M -> value_LF (get_here_LF M Gamma)
+| val_get_here_LF: forall M Ctx, value_LF M -> value_LF (get_here_LF Ctx M)
 .
 
 Global Reserved Notation " M |-> N " (at level 70).
 
-Inductive step_LF: (te_LF * Context_LF * Background_LF) -> (te_LF * Context_LF * Background_LF) -> Prop :=
+Inductive step_LF: (te_LF * ctx_LF) -> (te_LF * ctx_LF) -> Prop :=
 
-| red_appl_lam_LF: forall G Gamma M A N,
-  (appl_LF (lam_LF A M) N, Gamma, G) |-> 
-    ([N//0 | Gamma][M | Gamma], Gamma, G)
+| red_appl_lam_LF: forall ctx M A N,
+  (appl_LF (lam_LF A M) N, ctx) |-> 
+    ([N // 0] M, ctx)
 
-| red_unbox_box_LF: forall G Gamma M, (* ! ?added nil to G ! *)
-  (unbox_LF (box_LF M), Gamma, G) |-> 
-    (M, Gamma, G)
+| red_unbox_box_LF: forall ctx M,
+  (unbox_LF (box_LF M), ctx) |-> 
+    (M ^^ ctx, ctx)
 
-| red_unbox_fetch_box_LF: forall G Gamma Gamma' M, (* ! ?added nil to G ! *)
-  (unbox_fetch_LF (box_LF M) Gamma', Gamma, G) |-> 
-    (M, Gamma, G) 
+| red_unbox_fetch_box_LF: forall ctx ctx' M,
+  (unbox_fetch_LF ctx' (box_LF M), ctx) |-> 
+    (M ^^ ctx, ctx) 
 
-| red_letdia_here_LF: forall G Gamma M N A,
-  G |= Gamma |- here_LF M ::: <*>A ->
-  (letdia_LF (here_LF M) N, Gamma, G) |-> 
-    ([M // 0 | (A::nil)][N | Gamma], Gamma, G)
+| red_letdia_here_LF: forall ctx M N,
+  (letdia_LF (here_LF M) N, ctx) |-> 
+    ([M // 0] N ^^ ctx , ctx)
 
-| red_letdia__get_here_LF: forall G Gamma Gamma' M N A,
-  G |= Gamma |- get_here_LF M Gamma' ::: <*> A ->
-  (letdia_LF (get_here_LF M Gamma') N, Gamma, G) |-> 
-    ([M // 0 | (A::nil)][N | Gamma] , Gamma, G)
+| red_letdia__get_here_LF: forall ctx ctx' M N,
+  (letdia_LF (get_here_LF ctx' M) N, ctx) |-> 
+    ([M // 0] N ^^ ctx, ctx)
 
-| red_letdia_get__here_LF: forall G G' Gamma Gamma' M N A,
-  permut (G' & Gamma') (G & Gamma) ->
-  G' |= Gamma' |- here_LF M ::: <*> A ->
-  (letdia_get_LF (here_LF M) N Gamma', Gamma, G) |-> 
-    ([M // 0 | (A::nil)][N | Gamma], Gamma, G)
+| red_letdia_get__here_LF: forall ctx ctx' M N,
+  (letdia_get_LF ctx' (here_LF M) N, ctx) |-> 
+    ([M // 0] N ^^ ctx , ctx)
 
-| red_letdia_get_get_here_LF: forall G G' Gamma Gamma' Delta M N A,
-  permut (G' & Gamma') (G & Gamma) ->
-  G' |= Gamma' |- get_here_LF M Delta ::: <*> A ->
-  (letdia_get_LF (get_here_LF M Delta) N Gamma', Gamma, G) |-> 
-    ([M // 0 | (A::nil)][N | Gamma], Gamma, G)
+| red_letdia_get_get_here_LF: forall ctx ctx' ctx'' M N,
+  (letdia_get_LF ctx' (get_here_LF ctx'' M) N, ctx) |-> 
+    ([M // 0] N ^^ ctx , ctx)
 
-| red_appl_LF: forall G Gamma M N M'
-  (HT: (M, Gamma, G) |-> (M', Gamma, G)), 
-  (appl_LF M N, Gamma, G) |-> (appl_LF M' N, Gamma, G)
+| red_appl_LF: forall ctx M N M'
+  (HT: (M, ctx) |-> (M', ctx)), 
+  (appl_LF M N, ctx) |-> (appl_LF M' N, ctx)
 
-| red_unbox_LF: forall G Gamma M M'
-  (HT: (M, Gamma, G) |-> (M', Gamma, G)), 
-  (unbox_LF M, Gamma, G) |-> (unbox_LF M', Gamma, G)
+| red_unbox_LF: forall ctx M M'
+  (HT: (M, ctx) |-> (M', ctx)), 
+  (unbox_LF M, ctx) |-> (unbox_LF M', ctx)
 
-| red_unbox_fetch_LF: forall G G' Gamma' M M' Gamma
-(*
-  (HPermutG': permut G' (G & Gamma'))
-  (HPermutG'': permut G'' (G & Gamma))
-*)
-  (HT: (M, Gamma', G') |-> (M', Gamma', G')), 
-  (unbox_fetch_LF M Gamma', Gamma, G) |-> (unbox_fetch_LF M' Gamma', Gamma, G)
+| red_unbox_fetch_LF: forall ctx' M M' ctx
+  (HT: (M, ctx') |-> (M', ctx')), 
+  (unbox_fetch_LF ctx' M, ctx) |-> (unbox_fetch_LF ctx' M', ctx)
 
-| red_here_LF: forall G Gamma M M' 
-  (HT: (M, Gamma, G) |-> (M', Gamma, G)), 
-  (here_LF M, Gamma, G) |-> (here_LF M', Gamma, G)
+| red_here_LF: forall ctx M M' 
+  (HT: (M, ctx) |-> (M', ctx)), 
+  (here_LF M, ctx) |-> (here_LF M', ctx)
 
-| red_get_here_LF: forall G  G' Gamma Gamma' M M' 
-(*
-  (HPermutG': permut G' (G & Gamma'))
-  (HPermutG'': permut G'' (G & Gamma))
-*)
-  (HT: (M, Gamma, G') |-> (M', Gamma, G')), 
-  (get_here_LF M Gamma, Gamma', G) |-> (get_here_LF M' Gamma, Gamma', G)
+| red_get_here_LF: forall ctx ctx' M M' 
+  (HT: (M, ctx) |-> (M', ctx)), 
+  (get_here_LF ctx M, ctx') |-> (get_here_LF ctx M', ctx')
 
-| red_letdia_LF: forall G Gamma M N M' 
-  (HT: (M, Gamma, G) |-> (M', Gamma, G)),
-  (letdia_LF M N, Gamma, G) |-> (letdia_LF M' N, Gamma, G)
+| red_letdia_LF: forall ctx M N M' 
+  (HT: (M, ctx) |-> (M', ctx)),
+  (letdia_LF M N, ctx) |-> (letdia_LF M' N, ctx)
 
-| red_letdia_move_LF: forall G G' Gamma Gamma' M N M'
-(*
-  (HPermutG': permut G' (G & Gamma'))
-  (HPermutG'': permut G'' (G & Gamma)) 
-*)
-  (HT: (M, Gamma, G') |-> (M', Gamma, G')), 
-  (letdia_get_LF M N Gamma, Gamma', G) |-> (letdia_get_LF M' N Gamma, Gamma', G)
+| red_letdia_get_LF: forall ctx ctx' M N M'
+  (HT: (M, ctx) |-> (M', ctx)), 
+  (letdia_get_LF ctx M N, ctx') |-> (letdia_get_LF ctx M' N, ctx')
 
 where " M |-> N " := (step_LF M N ) : label_free_is5_scope.
 
+
 Section Lemmas.
 
-(* TODO: this may be moved to a separate file *)
-(* Permutation *)
-
-(* TODO *)
-Lemma PermutLastSame:
-forall A G G' (elem:A),
-  permut (G & elem) (G' & elem)
-  <->
-  permut G G'.
-Admitted.
-
-(* TODO *)
-Lemma PermutationElementSplit_Neq:
-forall A G G' H (elem:A) (elem':A)
-  (HNeq: elem <> elem')
-  (HT: permut (G & elem ++ G') (H & elem')),
-  exists GH, exists GT, H = GH & elem ++ GT.
-Admitted.
-
-(* TODO: not automated enough *)
-Lemma BackgroundSubsetImpl:
-forall G G' Gamma M A
-  (HT: G |= Gamma |- M ::: A)
-  (HSubst: exists GT, permut (G++GT) G'),
-  G' |= Gamma |- M ::: A.
-intros;
-generalize dependent G';
-induction HT; intros; eauto using types_LF.
-(* box *)
-destruct HSubst as [GT];
-constructor;
-apply IHHT;
-exists GT; permut_simpl; assumption.
-(* unbox_fetch *)
-destruct HSubst as [GT];
-apply t_unbox_fetch_LF with (Gamma:=Gamma) (G:=G++GT).
-apply IHHT;
-  exists GT; permut_simpl.
-apply permut_trans with (l2:= G' ++ GT); 
-[ permut_simpl | ]; assumption.
-(* get_here *)
-destruct HSubst as [GT];
-apply t_get_here_LF with (Gamma:=Gamma) (G:=G++GT).
-apply IHHT;
-  exists GT; permut_simpl.
-apply permut_trans with (l2:= G0 ++ GT); 
-[ permut_simpl | ]; assumption.
-(* letdia *)
-apply t_letdia_LF with (A:=A). 
-apply IHHT1; assumption.
-apply IHHT2; destruct HSubst as [GT];
-exists GT; permut_simpl; assumption.
-(* letdia_get *)
-destruct HSubst as [GT];
-apply t_letdia_get_LF with (A:=A)(Gamma:=Gamma) (G:=G++GT).
-apply IHHT1;
-  exists GT; permut_simpl.
-apply IHHT2;
-  exists GT; permut_simpl.
-apply permut_trans with (l2:= G0 ++ GT); 
-[ permut_simpl | ]; assumption.
-Qed.
-
 Lemma GlobalWeakening:
-forall G G' Gamma M A Ctx
-  (HT: G ++ G' |= Gamma |- M ::: A),
-  G & Ctx ++ G' |= Gamma |- M ::: A.
-intros; rew_app;
-apply BackgroundSubsetImpl with (G:=G++G');
-[assumption | exists (Ctx::nil); permut_simpl].
-Qed.
-
-(* When we have e.g. unbox_fetch M' Gamma and we weaken Gamma into Gamma++Delta, 
-   we need to change the term as well *)
-
-Reserved Notation " {{ A ~> B }} M " (at level 70).  
-Reserved Notation " }} A ~> B {{ [ M | C ] " (at level 70).
-
-Fixpoint inner_term_weakening (M: te_LF) (Gamma: Context_LF) (Delta: Context_LF) :=
-match M with
-| hyp_LF n => hyp_LF n
-| lam_LF A M' => lam_LF A ({{ Delta ~> A::Gamma}} M')
-| appl_LF M' N => appl_LF ({{Delta ~> Gamma}} M') ({{Delta ~> Gamma}} N)
-| box_LF M' => box_LF (}}Delta ~> Gamma{{ [ M' | nil ] )
-| unbox_LF M' => unbox_LF ({{Delta ~> Gamma}} M')
-| unbox_fetch_LF M' Gamma' => unbox_fetch_LF (}}Delta ~> Gamma{{ [M' | Gamma']) Gamma'
-| here_LF M' => here_LF ({{Delta ~> Gamma}} M') 
-| get_here_LF M' Gamma' => get_here_LF (}}Delta ~> Gamma{{ [M' | Gamma']) Gamma'
-| letdia_LF M' N => letdia_LF ({{Delta ~> Gamma}} M') ({{Delta ~> Gamma}} N)
-| letdia_get_LF M' N Gamma' =>
-  letdia_get_LF (}}Delta ~> Gamma{{ [M' | Gamma']) ({{Delta ~> Gamma}} N) Gamma'
-end
-where " {{ A ~> B }} M " := (inner_term_weakening M B A)
-with
-outer_term_weakening  (M: te_LF) (Gamma: Context_LF) (Gamma': Context_LF) (Delta: Context_LF) :=
-match M with
-| hyp_LF n => hyp_LF n
-| lam_LF A M' => lam_LF A (}}Delta ~> Gamma'{{ [M'| A::Gamma])
-| appl_LF M' N => 
-  appl_LF (}} Delta ~> Gamma'{{ [M'| Gamma]) (}}Delta ~> Gamma'{{ [N | Gamma])
-| box_LF M' => box_LF (}} Delta ~> Gamma'{{ [M' | nil])
-(*
-  match eq_context_LF_dec Gamma' nil with
-    | left _ => box_LF ({{Delta ~> nil}} M')
-    | right _ => box_LF (}}Delta ~> Gamma'{{ [M' | nil])
-  end
-*)
-| unbox_LF M' => unbox_LF (}}Delta ~> Gamma'{{ [M' | Gamma])
-| unbox_fetch_LF M' Gamma'' =>
-  match eq_context_LF_dec Gamma' Gamma'' with
-    | left _ => unbox_fetch_LF ({{Delta ~> Gamma''}} M') (Gamma''++Delta)
-    | right _ => unbox_fetch_LF (}}Delta ~> Gamma'{{ [M' | Gamma'']) Gamma''
-  end
-| here_LF M' => here_LF (}}Delta ~> Gamma'{{ [M' | Gamma]) 
-| get_here_LF M' Gamma'' => 
-  match eq_context_LF_dec Gamma' Gamma'' with
-    | left _ => get_here_LF ({{Delta ~> Gamma''}} M') (Gamma''++Delta)
-    | right _ => get_here_LF (}}Delta ~> Gamma'{{ [M' | Gamma'']) Gamma''
-  end
-| letdia_LF M' N => 
-  letdia_LF (}}Delta ~> Gamma'{{ [M' | Gamma]) (}}Delta ~> Gamma'{{ [N | Gamma])
-| letdia_get_LF M' N Gamma'' =>
-  match eq_context_LF_dec Gamma' Gamma'' with
-    | left _ => 
-      letdia_get_LF ({{Delta ~> Gamma''}} M') 
-                    (}}Delta ~> Gamma'{{ [N | Gamma]) (Gamma''++Delta)
-    | right _ =>  
-      letdia_get_LF (}}Delta ~> Gamma'{{ [M' | Gamma''])
-                    (}}Delta ~> Gamma'{{ [N | Gamma]) Gamma''
-  end
-end
-where " }} A ~> B {{ [ M | C ] " := (outer_term_weakening M C B A).
-
-(* TODO: ugly!!!... *)
-Lemma Weakening_general:
-  forall G Gamma M A
-  (HT: G |= Gamma |- M ::: A),
-  (forall G' Delta Delta',
-    permut G (G' & Delta) ->
-    G' & (Delta ++ Delta') |= Gamma |- (}}Delta' ~> Delta{{ [M | Gamma]) ::: A) /\ 
-  (forall Gamma',
-    G |= Gamma ++ Gamma' |- ({{Gamma' ~> Gamma}}M) ::: A).
-intros;
-induction HT; split;
-intros; subst; simpl.
-(* hyp *)
-eauto using types_LF.
-constructor; generalize dependent v_n;
-induction Gamma; destruct v_n; intros;
-try (apply Nth_nil_inv in HT; contradiction);
-apply Nth_app_l; assumption.
-(* lam *)
-constructor; eapply IHHT; eauto.
-constructor; eapply IHHT; eauto.
-(* appl *)
-econstructor; [eapply IHHT1| eapply IHHT2]; eauto.
-econstructor; [eapply IHHT1| eapply IHHT2]; eauto.
-(* box 1 *)
-constructor;
-apply BackgroundSubsetImpl with (G:=G' & Gamma & (Delta ++ Delta')).
-  eapply IHHT.
-    permut_simpl; assumption.
-  exists nil; permut_simpl; assumption.
-(* box 2 *)
-constructor;
-apply IHHT; permut_simpl.
-(* unbox *)
-constructor; apply IHHT; assumption.
-constructor; apply IHHT; assumption.
-(* unbox_fetch 1 *)
-destruct (eq_context_LF_dec Delta Gamma).
-(* = *)
-subst.
-apply t_unbox_fetch_LF with (G:=G).
-  apply IHHT.
-  apply permut_app_l;
-  apply PermutLastSame with (elem:=Gamma);
-  apply permut_trans with (l2:=G'); assumption.
-(* <> *)
-assert (exists G0, exists G1, G'0 = G0 & Gamma ++ G1).
-  apply PermutationElementSplit_Neq with (G:=G) (G':=nil) (elem':=Delta).
-    intro e; symmetry in e; contradiction.
-    rew_app; apply permut_trans with (l2:=G'); assumption.
-destruct H1 as [GH]; destruct H1 as [GT]; subst G'0.
-apply t_unbox_fetch_LF with (Gamma:=Gamma) (G:=GH ++ GT & (Delta ++ Delta')).
-apply BackgroundSubsetImpl with (G:= (GH ++ GT & Gamma') & (Delta ++ Delta')).
-  apply IHHT; permut_simpl.
-  apply PermutLastSame with (elem := Gamma).
-  apply permut_trans with (l2:=G').
-    assumption.
-    apply permut_trans with (l2:=(GH & Gamma ++ GT) & Delta).
-      assumption.
-      permut_simpl.
-  exists nil; permut_simpl.
-permut_simpl.
-(* unbox_fetch 2 *)
-apply t_unbox_fetch_LF with (G:=G) (Gamma:=Gamma).
-  apply IHHT; permut_simpl.
-  assumption.
-(* here *)
-constructor; apply IHHT; assumption.
-constructor; apply IHHT; assumption.
-(* get_here 1 *)
-destruct (eq_context_LF_dec Delta Gamma).
-(* = *)
-subst;
-apply t_get_here_LF with (Gamma:=Gamma++Delta') (G:=G).
-  apply IHHT.
-  apply permut_app_l;
-  apply PermutLastSame with (elem:=Gamma);
-  apply permut_trans with (l2:=G0); assumption.
-(* <> *)
-assert (exists G0, exists G1, G' = G0 & Gamma ++ G1).
-  apply PermutationElementSplit_Neq with (G:=G) (G':=nil) (elem':=Delta).
-    intro e; symmetry in e; contradiction.
-    rew_app; apply permut_trans with (l2:=G0); assumption.
-destruct H1 as [GH]; destruct H1 as [GT]; subst G';
-apply t_get_here_LF with (Gamma:=Gamma) (G:=GH ++ GT & (Delta ++ Delta')).
-apply BackgroundSubsetImpl with (G:= (GH ++ GT & Gamma') & (Delta ++ Delta')).
-  apply IHHT; permut_simpl;
-  apply PermutLastSame with (elem := Gamma);
-  apply permut_trans with (l2:=G0).
-    assumption.
-    apply permut_trans with (l2:=(GH & Gamma ++ GT) & Delta).
-      assumption.
-      permut_simpl.
-  exists nil; permut_simpl.
-permut_simpl.
-(* get_here 2 *)
-apply t_get_here_LF with (G:=G) (Gamma:=Gamma).
-  apply IHHT; permut_simpl.
-  assumption.
-(* letdia *)
-apply t_letdia_LF with (A:=A).
-apply IHHT1; assumption.
-apply IHHT2 with (G':=(A::nil)::G');
-permut_simpl;
-assumption.
-apply t_letdia_LF with (A:=A).
-apply IHHT1; assumption.
-apply IHHT2. 
-(* letdia_get 1 *)
-destruct (eq_context_LF_dec Delta Gamma).
-(* = *)
-subst;
-apply t_letdia_get_LF with (A:=A)(Gamma:=Gamma++Delta') (G:=G).
-apply IHHT1; assumption.
-apply BackgroundSubsetImpl with (G:=((A::nil) :: G) & (Gamma ++ Delta')).
-  apply IHHT2; permut_simpl.
-  exists nil; permut_simpl.
-apply permut_app_l;
-apply PermutLastSame with (elem:=Gamma);
-apply permut_trans with (l2:=G0); assumption.
-(* <> *)
-assert (exists G0, exists G1, G' = G0 & Gamma ++ G1).
-  apply PermutationElementSplit_Neq with (G:=G) (G':=nil) (elem':=Delta).
-    intro e; symmetry in e; contradiction.
-    rew_app; apply permut_trans with (l2:=G0); assumption.
-destruct H1 as [GH]; destruct H1 as [GT];
-subst G';
-apply t_letdia_get_LF with (A:=A)(Gamma:=Gamma) (G:=GH ++ GT & (Delta ++ Delta')).
-(* <*> A*)
-apply BackgroundSubsetImpl with (G:= (GH ++ GT & Gamma') & (Delta ++ Delta')).
-  apply IHHT1;
-  permut_simpl;
-  apply PermutLastSame with (elem := Gamma);
-  apply permut_trans with (l2:=G0).
-    assumption.
-    apply permut_trans with (l2:=(GH & Gamma ++ GT) & Delta).
-      assumption.
-      permut_simpl.
-exists nil; permut_simpl.
-(* B *)
-apply BackgroundSubsetImpl with (G:=(((A :: nil) :: GH ++ GT & Gamma) & (Delta ++ Delta'))).
-  apply IHHT2;
-  permut_simpl;
-  apply PermutLastSame with (elem := Gamma);
-  apply permut_trans with (l2:=G0).
-    assumption. 
-    permut_simpl.
-    apply permut_trans with (l2:=(GH & Gamma ++ GT) & Delta).
-      assumption.
-      permut_simpl.
-  exists nil; permut_simpl.
-permut_simpl.
-(* letdia_get 2 *)
-apply t_letdia_get_LF with (A:=A)(G:=G) (Gamma:=Gamma).
-apply IHHT1; permut_simpl.
-apply IHHT2; permut_simpl.
-assumption.
-Qed.
+forall G G' Ctx Ctx' M A
+  (HT: G ++ G' |= Ctx |- M ::: A),
+  G & Ctx' ++ G' |= Ctx |- M ::: A.
+Admitted.
 
 Lemma WeakeningBackgroundElem:
-forall G G' Delta Delta' Gamma M A
-  (HT: G & Delta ++ G' |= Gamma |- M ::: A),
-  G & (Delta ++ Delta') ++ G' |= Gamma |- }} Delta' ~> Delta{{ [M | Gamma] ::: A.
-intros.
-apply BackgroundSubsetImpl with (G:=(G++G') & (Delta ++ Delta')).
-assert (permut (G & Delta ++ G') ((G++G') & Delta)).
-  permut_simpl.
-eapply Weakening_general; eassumption.
-exists nil; permut_simpl.
-Qed.
+forall G G' w Delta Delta' Ctx M A
+  (HT: G & (w, Delta) ++ G' |= Ctx |- M ::: A),
+  G & (w, Delta ++ Delta') ++ G' |= Ctx |- M ::: A.
+Admitted.
 
 Lemma Weakening:
-forall G Gamma Gamma' M A
-  (HT: G |= Gamma |- M ::: A),
-  G |= Gamma ++ Gamma' |- {{Gamma' ~> Gamma}}M ::: A.
-intros;
-eapply Weakening_general; eassumption.
-Qed.
+forall G w Gamma Gamma' M A
+  (HT: G |= (w, Gamma) |- M ::: A),
+  G |= (w, Gamma ++ Gamma') |- M ::: A.
+Admitted.
 
-Lemma Progress:
-forall G M A
-  (EmptyCtx: forall G', 
-    permut G G' -> 
-    forall Ctx, Mem Ctx G' -> Ctx = nil)
-  (HT: G |= nil |- M ::: A),
-  value_LF M \/ exists N, (M, nil, G) |-> (N, nil, G).
-induction M; intros; eauto using value_LF.
-(* hyp *)
-inversion HT; destruct n;
-apply Nth_nil_inv in HT0; contradiction.
-(* appl *)
-right; inversion HT; subst;
-destruct (IHM1 (A0 ---> A) EmptyCtx HT1).
-  inversion H; subst; inversion HT1; subst; eexists; constructor.
-  destruct H; eexists; constructor; eapply H.
-(* unbox *)
-right; inversion HT; subst;
-destruct (IHM ([*]A) EmptyCtx HT0).
-  inversion H; subst; inversion HT0; subst; eexists; constructor.
-  destruct H; eexists; constructor; eapply H.
-(* unbox_fetch *)
-right; inversion HT; subst.
-assert (c = nil).
-  apply EmptyCtx with (G':=G0 & c).
-  apply permut_sym; assumption.
-  rewrite Mem_app_or_eq; right; rewrite Mem_cons_eq; left; reflexivity.
-subst; destruct (IHM ([*]A) EmptyCtx).
-apply BackgroundSubsetImpl with (G:=G0 & nil). 
-assumption.
-exists nil; rew_app; assumption.
-inversion H; subst; inversion HT0; subst; eexists; constructor.
-destruct H as [M'].
-exists (unbox_fetch_LF M' nil). 
-apply red_unbox_fetch_LF with (G':=G).
-assumption.
-(* here *)
-inversion HT; subst.
-destruct (IHM A0 EmptyCtx HT0).
-left; apply val_here_LF; assumption.
-right; destruct H; exists (here_LF x); eauto using step_LF.
-(* get_here *)
-inversion HT; subst.
-assert (c = nil).
-  apply EmptyCtx with (G' := G0 & c).
-  apply permut_sym; assumption.
-  rewrite Mem_app_or_eq; right;
-  rewrite Mem_cons_eq; left; reflexivity.
-subst; destruct (IHM A0 EmptyCtx).
-apply BackgroundSubsetImpl with (G:=G0 & nil).
-assumption.
-exists nil; permut_simpl; assumption.
-left; econstructor; eassumption.
-right; destruct H as [x]; exists (get_here_LF x nil);
-apply red_get_here_LF with (G':=G); assumption.
-(* letdia *)
-right; inversion HT; subst.
-destruct (IHM1 (<*>A0) EmptyCtx HT1).
-inversion H; subst; inversion HT1; subst.
-  exists ([M//0 | A0::nil][M2 | nil]);
-  apply red_letdia_here_LF; assumption.
-  exists ([M//0 | A0::nil][M2 | nil]);
-  apply red_letdia__get_here_LF; assumption.
-destruct H; exists (letdia_LF x M2); eauto using step_LF.
-(* letdia_get *)
-right; inversion HT; subst.
-assert (c = nil).
-  apply EmptyCtx with (G' := G0 & c).
-  apply permut_sym; assumption.
-  rewrite Mem_app_or_eq; right;
-  rewrite Mem_cons_eq; left; reflexivity.
-subst; destruct (IHM1 (<*>A0) EmptyCtx).
-apply BackgroundSubsetImpl with (G:=G0 & nil).
-assumption.
-exists nil; permut_simpl; assumption.
-inversion H; subst; inversion HT1; subst.
-  exists ([M//0 | A0::nil][M2 | nil]).
-  apply red_letdia_get__here_LF with (G':=G0&nil).
-    apply permut_app_l; assumption.
-    assumption.
-  exists ([M//0 | A0::nil][M2 | nil]).
-  apply red_letdia_get_get_here_LF with (G':=G0&nil).
-    apply permut_app_l; assumption.
-    assumption.
-destruct H as [x];
-exists (letdia_get_LF x M2 nil); 
-eauto using step_LF.
-Qed.
 
 (* Original formulations of modified typing rules can be reconstructed *)
 Lemma test_box:
-  forall G G' Gamma M A,
-    G & Gamma ++ G' |=  nil |- M ::: A ->
-      G ++ G' |= Gamma |- box_LF M ::: [*]A.
-intros; constructor;
-apply BackgroundSubsetImpl with (G:=G & Gamma ++ G');
-[ assumption | exists nil; permut_simpl].
-Qed.
+  forall L G G' Ctx M A,
+    forall w', w' \notin L -> 
+      G & Ctx ++ G' |=  (w', nil) |- M^^(fctx w') ::: A ->
+      G ++ G' |= Ctx |- box_LF M ::: [*]A.
+Admitted.
 
 Lemma test_unbox_fetch:
-  forall G G' Gamma Gamma' M A,
-    G & Gamma ++ G' |= Gamma' |- M ::: [*] A ->
-      G & Gamma' ++ G' |= Gamma |- unbox_fetch_LF M Gamma' ::: A.
-intros;
-apply t_unbox_fetch_LF with (G:=G ++ G') (Gamma:=Gamma');
-[apply BackgroundSubsetImpl with (G:=G & Gamma ++ G') | permut_simpl];
-[ assumption | exists nil; permut_simpl].
-Qed.
+  forall G G' Ctx w' Gamma' M A,
+    G & Ctx ++ G' |= (w', Gamma') |- M ::: [*] A ->
+      G & (w', Gamma') ++ G' |= Ctx |- unbox_fetch_LF (fctx w') M ::: A.
+Admitted.
 
 Lemma test_get_here:
-  forall G G' Gamma Gamma' M A,
-    G & Gamma' ++ G' |= Gamma |- M ::: A ->
-      G & Gamma ++ G' |= Gamma' |- get_here_LF M Gamma ::: <*> A.
-intros;
-apply t_get_here_LF with (G:=G ++ G') (Gamma:=Gamma);
-[apply BackgroundSubsetImpl with (G:=G & Gamma' ++ G') | permut_simpl];
-[assumption | exists nil; permut_simpl].
-Qed.
+  forall G G' Ctx w' Gamma' M A,
+    G & Ctx ++ G' |= (w', Gamma') |- M ::: A ->
+      G & (w', Gamma') ++ G' |= Ctx |- get_here_LF (fctx w') M ::: <*> A.
+Admitted.
 
 Lemma test_letdia_get:
-  forall G G' Gamma Gamma' M N A B,
-    G & Gamma' ++ G' |= Gamma |- M ::: <*>A ->
-    (A::nil) :: G & Gamma ++ G' |= Gamma' |- N ::: B ->
-      G & Gamma ++ G' |= Gamma' |-  letdia_get_LF M N Gamma ::: B.
-intros;
-apply t_letdia_get_LF with (A:=A) (Gamma:=Gamma) (G:=G ++ G');
-[ apply BackgroundSubsetImpl with (G:=G & Gamma' ++ G') |
-  apply BackgroundSubsetImpl with (G:=(A::nil) :: G & Gamma ++ G') |
-  permut_simpl];
-  [assumption | exists nil; permut_simpl |
-   assumption | exists nil; permut_simpl ].
-Qed.
+  forall L G G' Ctx w' Gamma' M N A B,
+    G & (w', Gamma') ++ G' |= Ctx |- M ::: <*>A ->
+    forall w'', w'' \notin L -> 
+      (w'', (A::nil)) :: G & Ctx ++ G' |= (w', Gamma') |- N ^^ (fctx w'') ::: B ->
+      G & Ctx ++ G' |= (w', Gamma') |-  letdia_get_LF (fctx w') M N ::: B.
+Admitted.
+
+(* / *)
+
+Fixpoint emptyEquiv (G: Background_LF) : Background_LF :=
+match G with
+| nil => nil
+| (w, a)::G => (w, nil) :: emptyEquiv G
+end.
+
+Lemma Progress:
+forall G w M A
+  (HT: emptyEquiv G |= (w, nil) |- M ::: A),
+  value_LF M \/ exists N, (M, fctx w) |-> (N, fctx w).
+Admitted.
+
+Lemma Preservation:
+forall G w M N A
+  (HT: emptyEquiv G |= (w, nil) |- M ::: A)
+  (HS: (M, fctx w) |-> (N, fctx w)),
+  emptyEquiv G |= (w, nil) |- N ::: A.
+Admitted.
 
 End Lemmas.
 
