label-free/Substitution.v
@@ -4,79 +4,73 @@ Require Import List.
 
 Open Scope label_free_is5_scope.
 
-Reserved Notation " [ M // x  | CtxSubst ] [ N | CtxCurr ] " (at level 5).
+Reserved Notation " {{ ctx1 // ctx2 }} Gamma " (at level 5).
 
-(* "outer" substitution - current context is not the one in which we want to substitute *)
-Fixpoint find_subst (M: te_LF) (n: nat) (N: te_LF) (CtxSubst: Context_LF) (CtxCurr: Context_LF) {struct N} : te_LF :=
-match N with
-| hyp_LF n' => N
-| lam_LF A N' => lam_LF A (find_subst M n N' CtxSubst (A::CtxCurr))
-| appl_LF N1 N2 => 
-  appl_LF (find_subst M n N1 CtxSubst CtxCurr) (find_subst M n N2 CtxSubst CtxCurr)
-(* unsure  - maybe skip the matching? *)
-| box_LF N' => 
-  match (eq_context_LF_dec CtxSubst nil) with
-    | left _ => box_LF (inner_subst M n N' nil)
-    | right _ => box_LF (find_subst M n N' CtxSubst nil) 
+Fixpoint subst_ctx (M0 : te_LF) (ctx1: ctx_LF) (ctx2: ctx_LF) :=
+match M0 with 
+| hyp_LF n => hyp_LF n
+| lam_LF A M =>lam_LF A {{ctx1 // ctx2}} M
+| appl_LF M N => appl_LF {{ctx1 // ctx2}}M {{ctx1 // ctx2}}N
+| box_LF M => 
+  match ctx1, ctx2 with
+    | bctx c1, bctx c2 => box_LF {{bctx (S c1) // bctx (S c2)}} M
+    | bctx c1, fctx c2 => box_LF {{bctx (S c1) // ctx2}} M
+    | fctx c1, bctx c2 => box_LF {{ctx1 // bctx (S c2)}} M
+    | fctx c1, fctx c2 => box_LF {{ctx1 // ctx2}} M
   end
-| unbox_LF N' => unbox_LF (find_subst M n N' CtxSubst CtxCurr)
-| unbox_fetch_LF N' CtxSwitch => 
-  match (eq_context_LF_dec CtxSubst CtxSwitch) with
-    | left _ => unbox_fetch_LF (inner_subst M n N' CtxSwitch) CtxSwitch
-    | right _ => unbox_fetch_LF (find_subst M n N' CtxSubst CtxSwitch) CtxSwitch
+| unbox_LF M => unbox_LF {{ctx1 // ctx2}} M
+| unbox_fetch_LF ctx M =>
+  let ctx' := if eq_ctx_LF_dec ctx ctx2 then ctx1 else ctx in
+  unbox_fetch_LF ctx' {{ctx1 // ctx2}} M
+| here_LF M => here_LF {{ctx1 // ctx2}} M
+| get_here_LF ctx M =>
+  let ctx' := if eq_ctx_LF_dec ctx ctx2 then ctx1 else ctx in
+  get_here_LF ctx' {{ctx1 // ctx2}}M
+| letdia_LF M N =>
+  match ctx1, ctx2 with
+    | bctx c1, bctx c2 => letdia_LF {{ctx1 // ctx2}}M {{bctx (S c1) // bctx (S c2)}}N
+    | bctx c1, fctx c2 => letdia_LF {{ctx1 // ctx2}}M {{bctx (S c1) // ctx2}}N
+    | fctx c1, bctx c2 => letdia_LF {{ctx1 // ctx2}}M {{ctx1 // bctx (S c2)}}N
+    | fctx c1, fctx c2 => letdia_LF {{ctx1 // ctx2}}M {{ctx1 // ctx2}}N
   end
-| here_LF N' => here_LF (find_subst M n N' CtxSubst CtxCurr)
-| get_here_LF N' CtxSwitch => 
-  match (eq_context_LF_dec CtxSubst CtxSwitch) with
-    | left _ => get_here_LF (inner_subst M n N' CtxSwitch) CtxSwitch
-    | right _ => get_here_LF (find_subst M n N' CtxSubst CtxSwitch) CtxSwitch
-  end
-| letdia_LF N1 N2 => 
-  letdia_LF (find_subst M n N1 CtxSubst CtxCurr) (find_subst M n N2 CtxSubst CtxCurr)
-| letdia_get_LF N1 N2 CtxSwitch => 
-  match (eq_context_LF_dec CtxSubst CtxSwitch) with
-    | left _ => letdia_get_LF (inner_subst M n N1 CtxSwitch) 
-                              (find_subst M n N2 CtxSubst CtxCurr) CtxSwitch
-    | right _ => letdia_get_LF (find_subst M n N1 CtxSubst CtxSwitch) 
-                               (find_subst M n N2 CtxSubst CtxCurr) CtxSwitch
+| letdia_get_LF ctx M N =>
+  let ctx' := if eq_ctx_LF_dec ctx ctx2 then ctx1 else ctx in
+  match ctx1, ctx2 with
+    | bctx c1, bctx c2 => letdia_get_LF ctx' {{ctx1 // ctx2}}M {{bctx (S c1) // bctx (S c2)}}N
+    | bctx c1, fctx c2 => letdia_get_LF ctx' {{ctx1 // ctx2}}M {{bctx (S c1) // ctx2}}N
+    | fctx c1, bctx c2 => letdia_get_LF ctx' {{ctx1 // ctx2}}M {{ctx1 // bctx (S c2)}}N
+    | fctx c1, fctx c2 => letdia_get_LF ctx' {{ctx1 // ctx2}}M {{ctx1 // ctx2}}N
   end
 end
-with
-(* "inner" substitution - the usual substitution; when we change context, we go back to 
-   "outer" *)
-inner_subst (M: te_LF) (n: nat) (N: te_LF) (CtxCurr: Context_LF) {struct N} : te_LF :=
+where " {{ c1 // c2 }} M " := (subst_ctx M c1 c2) : label_free_is5_scope.
+
+Definition open_ctx M c := subst_ctx M c (bctx 0). 
+Notation " M ^^ Gamma " := (open_ctx M Gamma) (at level 5) : label_free_is5_scope.
+
+(* TODO: this may be too little - we may need "outer" substitution with context switch 
+         and in that case when moving between contexts we will use "outer" substitution
+         to find the next occ. of "our" context *)
+Reserved Notation " [ M // n ] N " (at level 5).
+
+Fixpoint subst_LF (M: te_LF) (n: nat) (N: te_LF) : te_LF :=
 match N with
-| hyp_LF n' => if (eq_nat_dec n n') then M else N
-| lam_LF A N' => lam_LF A (inner_subst M (S n) N' (A::CtxCurr))
-| appl_LF N1 N2 => appl_LF (inner_subst M n N1 CtxCurr) (inner_subst M n N2 CtxCurr)
-| box_LF N' => box_LF (find_subst M n N' CtxCurr nil)
-| unbox_LF N' => unbox_LF (inner_subst M n N' CtxCurr)
-| unbox_fetch_LF N' CtxSwitch => 
-  unbox_fetch_LF (find_subst M n N' CtxCurr CtxSwitch) CtxSwitch
-| here_LF N' => here_LF (inner_subst M n N' CtxCurr)
-| get_here_LF N' CtxSwitch => get_here_LF (find_subst M n N' CtxCurr CtxSwitch) CtxSwitch
-| letdia_LF N1 N2 => letdia_LF (inner_subst M n N1 CtxCurr) (inner_subst M n N2 CtxCurr)
-| letdia_get_LF N1 N2 CtxSwitch => 
-  letdia_get_LF (find_subst M n N1 CtxCurr CtxSwitch)
-                (inner_subst M n N2 CtxCurr) CtxSwitch 
-end.
+| hyp_LF n' => if eq_nat_dec n n' then M else N
+| lam_LF A N' => lam_LF A [M//S n] N'
+| appl_LF N1 N2 => appl_LF ([M // n] N1) ([M // n] N2)
+| box_LF N' => box_LF ([M // n] N')
+| unbox_LF N' => unbox_LF ([M // n] N')
+| unbox_fetch_LF Ctx N' => N
+| here_LF N' => here_LF ([M // n] N')
+| get_here_LF Ctx N' => N
+| letdia_LF N1 N2 => letdia_LF ([M // n] N1) ([M // S n ] N2)
+| letdia_get_LF Ctx N1 N2 => N
+end
+where " [ M // n ] N " := (subst_LF M n N) : label_free_is5_scope.
 
-Definition subst_LF (M:te_LF) (n:nat) (Delta: Context_LF) 
-                  (N:te_LF) (Gamma: Context_LF): te_LF := 
-match (eq_context_LF_dec Delta Gamma) with
-| left _ => inner_subst M n N Gamma
-| right _ => find_subst M n N Gamma Delta
-end.
-
-Notation " [ M // x | Delta ] [ N | Gamma ] " := (subst_LF M x Delta N Gamma) : label_free_is5_scope.
-
-
-(* Substitute L[0] for n, L[1] for n+1,.. in M *)
-(* unsure - maybe we should allow each substitution to have a different CtxSubst? *) 
-Fixpoint subst_list L n N CtxSubst CtxCurr :=
+Fixpoint subst_list L n N :=
 match L with
 | nil => N
-| M :: L' => [ M // n | CtxSubst] [(subst_list L' (S n) N CtxSubst CtxCurr) | CtxCurr]
+| M :: L' => [ M // n ] (subst_list L' (S n) N)
 end.
 
 Close Scope label_free_is5_scope.
